<?xml version="1.0"?>
<rdf:RDF xmlns="http://www.semanticweb.org/AdditiveManufacturingOntology#"
     xml:base="http://www.semanticweb.org/AdditiveManufacturingOntology"
     xmlns:dc="http://purl.org/dc/elements/1.1/"
     xmlns:cco="http://www.ontologyrepository.com/CommonCoreOntologies/"
     xmlns:obo="http://purl.obolibrary.org/obo/"
     xmlns:owl="http://www.w3.org/2002/07/owl#"
     xmlns:rdf="http://www.w3.org/1999/02/22-rdf-syntax-ns#"
     xmlns:xml="http://www.w3.org/XML/1998/namespace"
     xmlns:xsd="http://www.w3.org/2001/XMLSchema#"
     xmlns:rdfs="http://www.w3.org/2000/01/rdf-schema#"
     xmlns:skos="http://www.w3.org/2004/02/skos/core#"
     xmlns:dcterms="http://purl.org/dc/terms/">
    <owl:Ontology rdf:about="http://www.semanticweb.org/AdditiveManufacturingOntology">
        <owl:versionIRI rdf:resource="http://www.semanticweb.org/AdditiveManufacturingOntology"/>
        <owl:imports rdf:resource="http://www.ontologyrepository.com/CommonCoreOntologies/Mid/ExtendedRelationOntology"/>
        <owl:imports rdf:resource="https://raw.githubusercontent.com/BuffaloMfgWorks/AM-CDM-Ontology-Map/main/Imports/InformationEntityOntologyNoGEO.ttl"/>
        <owl:imports rdf:resource="https://raw.githubusercontent.com/BuffaloMfgWorks/AM-CDM-Ontology-Map/main/Imports/Manufacturing.owl"/>
    </owl:Ontology>
    


    <!-- 
    ///////////////////////////////////////////////////////////////////////////////////////
    //
    // Classes
    //
    ///////////////////////////////////////////////////////////////////////////////////////
     -->

    


    <!-- http://www.semanticweb.org/AdditiveManufacturingOntology/AMSubsystem -->

    <owl:Class rdf:about="http://www.semanticweb.org/AdditiveManufacturingOntology/AMSubsystem">
        <owl:equivalentClass>
            <owl:Class>
                <owl:intersectionOf rdf:parseType="Collection">
                    <rdf:Description rdf:about="http://www.semanticweb.org/AdditiveManufacturingOntology/System"/>
                    <owl:Restriction>
                        <owl:onProperty rdf:resource="http://purl.obolibrary.org/obo/BFO_0000196"/>
                        <owl:someValuesFrom rdf:resource="http://www.ontologyrepository.com/CommonCoreOntologies/ComponentRole"/>
                    </owl:Restriction>
                </owl:intersectionOf>
            </owl:Class>
        </owl:equivalentClass>
        <rdfs:subClassOf rdf:resource="http://www.semanticweb.org/AdditiveManufacturingOntology/System"/>
        <cco:definition>A System that bears some Component Role within an Additive Manufacturing System.</cco:definition>
        <rdfs:comment>This class represents subsystems within an Additive Manufacturing System, such as a laser system in a selective laser sintering machine or an extruder in a fused deposition modeling printer, which are essential for the system&apos;s operation and success in manufacturing processes.</rdfs:comment>
        <rdfs:label xml:lang="en">Additive Manufacturing Subsystem</rdfs:label>
    </owl:Class>
    


    <!-- http://www.semanticweb.org/AdditiveManufacturingOntology/AMSystem -->

    <owl:Class rdf:about="http://www.semanticweb.org/AdditiveManufacturingOntology/AMSystem">
        <owl:equivalentClass>
            <owl:Class>
                <owl:intersectionOf rdf:parseType="Collection">
                    <rdf:Description rdf:about="http://www.semanticweb.org/AdditiveManufacturingOntology/System"/>
                    <owl:Restriction>
                        <owl:onProperty rdf:resource="http://purl.obolibrary.org/obo/BFO_0000196"/>
                        <owl:someValuesFrom rdf:resource="http://www.semanticweb.org/AdditiveManufacturingOntology/AMSystemRole"/>
                    </owl:Restriction>
                </owl:intersectionOf>
            </owl:Class>
        </owl:equivalentClass>
        <owl:equivalentClass>
            <owl:Class>
                <owl:intersectionOf rdf:parseType="Collection">
                    <rdf:Description rdf:about="http://www.semanticweb.org/AdditiveManufacturingOntology/System"/>
                    <owl:Restriction>
                        <owl:onProperty rdf:resource="http://www.ontologyrepository.com/CommonCoreOntologies/agent_in"/>
                        <owl:someValuesFrom rdf:resource="http://www.semanticweb.org/AdditiveManufacturingOntology/ActOfAdditiveManufacturing"/>
                    </owl:Restriction>
                </owl:intersectionOf>
            </owl:Class>
        </owl:equivalentClass>
        <rdfs:subClassOf rdf:resource="http://www.semanticweb.org/AdditiveManufacturingOntology/System"/>
        <cco:definition>A System that is an agent in an Act Of Additive Manufacturing and is the bearer of some AM System Role.</cco:definition>
        <rdfs:comment>This class represents systems specifically designed to carry out additive manufacturing processes, often involving the deposition of materials layer by layer to form objects.</rdfs:comment>
        <rdfs:label xml:lang="en">Additive Manufacturing System</rdfs:label>
    </owl:Class>
    


    <!-- http://www.semanticweb.org/AdditiveManufacturingOntology/AMSystemRole -->

    <owl:Class rdf:about="http://www.semanticweb.org/AdditiveManufacturingOntology/AMSystemRole">
        <rdfs:subClassOf rdf:resource="http://www.ontologyrepository.com/CommonCoreOntologies/SystemRole"/>
        <cco:definition>A System Role that inheres in some object aggregate that, if realized, is realized when the system performs an Act Of Additive Manufacturing through the coordinated operation of its components.</cco:definition>
        <rdfs:comment>This role is designated for systems that facilitate the additive manufacturing process, ensuring the coordination and functionality of the system&apos;s components to produce objects through layer-by-layer material deposition.</rdfs:comment>
        <rdfs:label xml:lang="en">Additive Manufacturing System Role</rdfs:label>
    </owl:Class>
    


    <!-- http://www.semanticweb.org/AdditiveManufacturingOntology/ActOfAdditiveManufacturing -->

    <owl:Class rdf:about="http://www.semanticweb.org/AdditiveManufacturingOntology/ActOfAdditiveManufacturing">
        <owl:equivalentClass>
            <owl:Class>
                <owl:intersectionOf rdf:parseType="Collection">
                    <rdf:Description rdf:about="http://www.ontologyrepository.com/CommonCoreOntologies/ActOfManufacturing"/>
                    <owl:Restriction>
                        <owl:onProperty rdf:resource="http://www.ontologyrepository.com/CommonCoreOntologies/has_input"/>
                        <owl:someValuesFrom rdf:resource="http://www.semanticweb.org/AdditiveManufacturingOntology/PortionofFeedstock"/>
                    </owl:Restriction>
                </owl:intersectionOf>
            </owl:Class>
        </owl:equivalentClass>
        <rdfs:subClassOf rdf:resource="http://www.ontologyrepository.com/CommonCoreOntologies/ActOfManufacturing"/>
        <cco:definition>An Act Of Manufacturing that involves the deposition of successive layers of material to create an object, using a PortionofFeedstock as input.</cco:definition>
        <cco:example_of_usage>Examples include 3D printing processes such as Fused Deposition Modeling (FDM), Selective Laser Sintering (SLS), and Stereolithography (SLA).</cco:example_of_usage>
        <rdfs:comment>This process typically involves the use of digital models to direct machinery in the layer-by-layer addition of material, resulting in a three-dimensional object. It is distinct from subtractive manufacturing, which removes material to form an object.</rdfs:comment>
        <rdfs:label xml:lang="en">Act of Additive Manufacturing</rdfs:label>
    </owl:Class>
    


    <!-- http://www.semanticweb.org/AdditiveManufacturingOntology/AdditiveManufacturingBuildSite -->

    <owl:Class rdf:about="http://www.semanticweb.org/AdditiveManufacturingOntology/AdditiveManufacturingBuildSite">
        <owl:equivalentClass>
            <owl:Class>
                <owl:intersectionOf rdf:parseType="Collection">
                    <rdf:Description rdf:about="http://purl.obolibrary.org/obo/BFO_0000029"/>
                    <owl:Restriction>
                        <owl:onProperty rdf:resource="http://purl.obolibrary.org/obo/BFO_0000176"/>
                        <owl:someValuesFrom rdf:resource="http://www.semanticweb.org/AdditiveManufacturingOntology/BuildChamber"/>
                    </owl:Restriction>
                </owl:intersectionOf>
            </owl:Class>
        </owl:equivalentClass>
        <rdfs:subClassOf rdf:resource="http://purl.obolibrary.org/obo/BFO_0000029"/>
        <cco:definition xml:lang="en">a site within a build chamber where the additive manufacturing process occurs.</cco:definition>
        <rdfs:label xml:lang="en">Additive Manufacturing Build Site</rdfs:label>
    </owl:Class>
    


    <!-- http://www.semanticweb.org/AdditiveManufacturingOntology/AdditiveManufacturingFacility -->

    <owl:Class rdf:about="http://www.semanticweb.org/AdditiveManufacturingOntology/AdditiveManufacturingFacility">
        <rdfs:subClassOf rdf:resource="http://www.semanticweb.org/AdditiveManufacturingOntology/ManufacturingFacility"/>
        <cco:definition xml:lang="en">a manufacturing facility that is designed for the production of goods using some additive manufacturing act</cco:definition>
        <rdfs:comment xml:lang="en">Note that it is often the case that subtractive manufacturing often occurs at additive manufacturing facilities.</rdfs:comment>
    </owl:Class>
    


    <!-- http://www.semanticweb.org/AdditiveManufacturingOntology/BuildChamber -->

    <owl:Class rdf:about="http://www.semanticweb.org/AdditiveManufacturingOntology/BuildChamber">
        <rdfs:subClassOf rdf:resource="http://www.ontologyrepository.com/CommonCoreOntologies/Artifact"/>
        <cco:definition_source xml:lang="en">A build chamber is a material artifact that is designed to contain a site where some controlled manufacturing process occures</cco:definition_source>
        <rdfs:label xml:lang="en">Build Chamber</rdfs:label>
    </owl:Class>
    


    <!-- http://www.semanticweb.org/AdditiveManufacturingOntology/InSituMonitoringAct -->

    <owl:Class rdf:about="http://www.semanticweb.org/AdditiveManufacturingOntology/InSituMonitoringAct">
        <owl:equivalentClass>
            <owl:Class>
                <owl:intersectionOf rdf:parseType="Collection">
                    <rdf:Description rdf:about="http://www.ontologyrepository.com/CommonCoreOntologies/ActOfMeasuring"/>
                    <owl:Restriction>
                        <owl:onProperty rdf:resource="http://www.ontologyrepository.com/CommonCoreOntologies/is_part_of_process"/>
                        <owl:someValuesFrom rdf:resource="http://purl.obolibrary.org/obo/BFO_0000015"/>
                    </owl:Restriction>
                </owl:intersectionOf>
            </owl:Class>
        </owl:equivalentClass>
        <rdfs:subClassOf rdf:resource="http://www.ontologyrepository.com/CommonCoreOntologies/ActOfMeasuring"/>
        <cco:definition>An Act Of Measuring that is part of some second process and has as an agent some In-Situ Monitoring System.</cco:definition>
        <rdfs:comment>This class represents the act of continuous observation and measurement within various processes, such as manufacturing, scientific experiments, or environmental monitoring, providing immediate feedback and control.</rdfs:comment>
        <rdfs:label xml:lang="en">In-Situ Monitoring Act</rdfs:label>
    </owl:Class>
    


    <!-- http://www.semanticweb.org/AdditiveManufacturingOntology/InSituMonitoringSystem -->

    <owl:Class rdf:about="http://www.semanticweb.org/AdditiveManufacturingOntology/InSituMonitoringSystem">
        <owl:equivalentClass>
            <owl:Class>
                <owl:intersectionOf rdf:parseType="Collection">
                    <rdf:Description rdf:about="http://www.semanticweb.org/AdditiveManufacturingOntology/System"/>
                    <owl:Restriction>
                        <owl:onProperty rdf:resource="http://purl.obolibrary.org/obo/BFO_0000196"/>
                        <owl:someValuesFrom rdf:resource="http://www.ontologyrepository.com/CommonCoreOntologies/MeasurementArtifactFunction"/>
                    </owl:Restriction>
                </owl:intersectionOf>
            </owl:Class>
        </owl:equivalentClass>
        <owl:equivalentClass>
            <owl:Class>
                <owl:intersectionOf rdf:parseType="Collection">
                    <rdf:Description rdf:about="http://www.semanticweb.org/AdditiveManufacturingOntology/System"/>
                    <owl:Restriction>
                        <owl:onProperty rdf:resource="http://www.ontologyrepository.com/CommonCoreOntologies/agent_in"/>
                        <owl:someValuesFrom rdf:resource="http://www.semanticweb.org/AdditiveManufacturingOntology/InSituMonitoringAct"/>
                    </owl:Restriction>
                </owl:intersectionOf>
            </owl:Class>
        </owl:equivalentClass>
        <rdfs:subClassOf rdf:resource="http://www.semanticweb.org/AdditiveManufacturingOntology/System"/>
        <cco:definition>A System that is an agent in some In-Situ Monitoring Act and bears some quality control function.</cco:definition>
        <rdfs:comment>This class includes systems used for continuous observation and measurement within different processes, such as manufacturing, scientific experiments, or environmental monitoring, to provide immediate feedback and control.</rdfs:comment>
        <rdfs:label xml:lang="en">In-Situ Monitoring System</rdfs:label>
    </owl:Class>
    


    <!-- http://www.semanticweb.org/AdditiveManufacturingOntology/ManufacturingFacility -->

    <owl:Class rdf:about="http://www.semanticweb.org/AdditiveManufacturingOntology/ManufacturingFacility">
        <rdfs:subClassOf rdf:resource="http://www.ontologyrepository.com/CommonCoreOntologies/Factory"/>
        <cco:definition xml:lang="en">A factory that is designed for the production of goods</cco:definition>
    </owl:Class>
    


    <!-- http://www.semanticweb.org/AdditiveManufacturingOntology/MaterialArtifactPart -->

    <owl:Class rdf:about="http://www.semanticweb.org/AdditiveManufacturingOntology/MaterialArtifactPart">
        <owl:equivalentClass>
            <owl:Class>
                <owl:intersectionOf rdf:parseType="Collection">
                    <rdf:Description rdf:about="http://www.ontologyrepository.com/CommonCoreOntologies/Artifact"/>
                    <owl:Restriction>
                        <owl:onProperty rdf:resource="http://purl.obolibrary.org/obo/BFO_0000196"/>
                        <owl:someValuesFrom rdf:resource="http://www.ontologyrepository.com/CommonCoreOntologies/PartRole"/>
                    </owl:Restriction>
                </owl:intersectionOf>
            </owl:Class>
        </owl:equivalentClass>
        <rdfs:subClassOf rdf:resource="http://www.ontologyrepository.com/CommonCoreOntologies/Artifact"/>
        <cco:alternative_label xml:lang="en">Part</cco:alternative_label>
        <cco:definition xml:lang="en">A Material Artifact that bears some Part Role</cco:definition>
        <rdfs:label xml:lang="en">Material Artifact Part</rdfs:label>
    </owl:Class>
    


    <!-- http://www.semanticweb.org/AdditiveManufacturingOntology/PortionofBulkSolid -->

    <owl:Class rdf:about="http://www.semanticweb.org/AdditiveManufacturingOntology/PortionofBulkSolid">
        <rdfs:subClassOf rdf:resource="http://www.semanticweb.org/AdditiveManufacturingOntology/PortionofFeedstock"/>
        <cco:definition>A Portion Of Feedstock that consists of bulk solid material.</cco:definition>
        <rdfs:comment>This class represents a bulk solid form of feedstock used in manufacturing processes.</rdfs:comment>
        <rdfs:label xml:lang="en">Portion of Bulk Solid Feedstock</rdfs:label>
    </owl:Class>
    


    <!-- http://www.semanticweb.org/AdditiveManufacturingOntology/PortionofFeedstock -->

    <owl:Class rdf:about="http://www.semanticweb.org/AdditiveManufacturingOntology/PortionofFeedstock">
        <rdfs:subClassOf rdf:resource="http://www.ontologyrepository.com/CommonCoreOntologies/PortionOfMaterial"/>
        <cco:definition>A Portion Of Material that serves as input material in a manufacturing processes.</cco:definition>
        <rdfs:comment>This class represents any material portion used as feedstock in various manufacturing processes.</rdfs:comment>
        <rdfs:label xml:lang="en">Portion of Feedstock</rdfs:label>
    </owl:Class>
    


    <!-- http://www.semanticweb.org/AdditiveManufacturingOntology/PortionofPowder -->

    <owl:Class rdf:about="http://www.semanticweb.org/AdditiveManufacturingOntology/PortionofPowder">
        <rdfs:subClassOf rdf:resource="http://www.semanticweb.org/AdditiveManufacturingOntology/PortionofFeedstock"/>
        <cco:definition>A PortionOfFeedstock that consists of powder material.</cco:definition>
        <rdfs:comment>This class represents a powder form of feedstock used in additive manufacturing and other processes.</rdfs:comment>
        <rdfs:label xml:lang="en">Portion of Powder Feedstock</rdfs:label>
    </owl:Class>
    


    <!-- http://www.semanticweb.org/AdditiveManufacturingOntology/PortionofReusedFeedstock -->

    <owl:Class rdf:about="http://www.semanticweb.org/AdditiveManufacturingOntology/PortionofReusedFeedstock">
        <owl:equivalentClass>
            <owl:Class>
                <owl:intersectionOf rdf:parseType="Collection">
                    <rdf:Description rdf:about="http://www.semanticweb.org/AdditiveManufacturingOntology/PortionofFeedstock"/>
                    <owl:Restriction>
                        <owl:onProperty rdf:resource="http://www.ontologyrepository.com/CommonCoreOntologies/is_output_of"/>
                        <owl:someValuesFrom rdf:resource="http://www.ontologyrepository.com/CommonCoreOntologies/ActOfManufacturing"/>
                    </owl:Restriction>
                </owl:intersectionOf>
            </owl:Class>
        </owl:equivalentClass>
        <rdfs:subClassOf rdf:resource="http://www.semanticweb.org/AdditiveManufacturingOntology/PortionofFeedstock"/>
        <cco:definition>A Portion Of Feedstock that is a reused output from a previous Act Of Manufacturing.</cco:definition>
        <rdfs:comment>This class represents feedstock that has been reused from previous manufacturing processes.</rdfs:comment>
        <rdfs:label xml:lang="en">Portion of Reused Feedstock</rdfs:label>
    </owl:Class>
    


    <!-- http://www.semanticweb.org/AdditiveManufacturingOntology/PortionofWire -->

    <owl:Class rdf:about="http://www.semanticweb.org/AdditiveManufacturingOntology/PortionofWire">
        <rdfs:subClassOf rdf:resource="http://www.semanticweb.org/AdditiveManufacturingOntology/PortionofFeedstock"/>
        <cco:definition>A PortionOfFeedstock that consists of wire material.</cco:definition>
        <rdfs:comment>This class represents a wire form of feedstock used in manufacturing processes such as wire arc additive manufacturing.</rdfs:comment>
        <rdfs:label xml:lang="en">Portion of Wire Feedstock</rdfs:label>
    </owl:Class>
    


    <!-- http://www.semanticweb.org/AdditiveManufacturingOntology/Subsystem -->

    <owl:Class rdf:about="http://www.semanticweb.org/AdditiveManufacturingOntology/Subsystem">
        <owl:equivalentClass>
            <owl:Class>
                <owl:intersectionOf rdf:parseType="Collection">
                    <rdf:Description rdf:about="http://www.semanticweb.org/AdditiveManufacturingOntology/System"/>
                    <owl:Restriction>
                        <owl:onProperty rdf:resource="http://purl.obolibrary.org/obo/BFO_0000196"/>
                        <owl:someValuesFrom rdf:resource="http://www.ontologyrepository.com/CommonCoreOntologies/ComponentRole"/>
                    </owl:Restriction>
                </owl:intersectionOf>
            </owl:Class>
        </owl:equivalentClass>
        <rdfs:subClassOf rdf:resource="http://www.semanticweb.org/AdditiveManufacturingOntology/System"/>
        <cco:definition>A System that bears some Component Role.</cco:definition>
        <rdfs:comment>This class represents systems that function as components or parts of larger systems, providing specific functionalities within the larger context.</rdfs:comment>
        <rdfs:label xml:lang="en">Subsystem</rdfs:label>
    </owl:Class>
    


    <!-- http://www.semanticweb.org/AdditiveManufacturingOntology/SubtractiveManufacturingFacility -->

    <owl:Class rdf:about="http://www.semanticweb.org/AdditiveManufacturingOntology/SubtractiveManufacturingFacility">
        <rdfs:subClassOf rdf:resource="http://www.semanticweb.org/AdditiveManufacturingOntology/ManufacturingFacility"/>
        <cco:definition xml:lang="en">a manufacturing facility that is designed for the production of goods using some subtractive manufacturing act.</cco:definition>
    </owl:Class>
    


    <!-- http://www.semanticweb.org/AdditiveManufacturingOntology/System -->

    <owl:Class rdf:about="http://www.semanticweb.org/AdditiveManufacturingOntology/System">
        <owl:equivalentClass>
            <owl:Class>
                <owl:intersectionOf rdf:parseType="Collection">
                    <rdf:Description rdf:about="http://purl.obolibrary.org/obo/BFO_0000027"/>
                    <owl:Restriction>
                        <owl:onProperty rdf:resource="http://purl.obolibrary.org/obo/BFO_0000196"/>
                        <owl:someValuesFrom rdf:resource="http://www.ontologyrepository.com/CommonCoreOntologies/SystemRole"/>
                    </owl:Restriction>
                </owl:intersectionOf>
            </owl:Class>
        </owl:equivalentClass>
        <rdfs:subClassOf rdf:resource="http://purl.obolibrary.org/obo/BFO_0000027"/>
        <cco:definition>An object aggregate that bears a System Role.</cco:definition>
        <rdfs:comment>This class represents any organized assembly of components that work together to perform specific functions or achieve particular goals.</rdfs:comment>
        <rdfs:label xml:lang="en">System</rdfs:label>
    </owl:Class>


    <owl:Class rdf:about="http://www.semanticweb.org/AdditiveManufacturingOntology/BuildInterruption">
        <rdfs:subClassOf rdf:resource="http://purl.obolibrary.org/obo/BFO_0000015"/>
        <rdfs:subClassOf>
            <owl:Restriction>
                <owl:onProperty rdf:resource="http://www.ontologyrepository.com/CommonCoreOntologies/is_part_of_process"/>
                <owl:someValuesFrom rdf:resource="http://www.ontologyrepository.com/CommonCoreOntologies/ActOfManufacturing"/>
            </owl:Restriction>
        </rdfs:subClassOf>
        <cco:definition xml:lang="en">A process that is part of an Act of Manufacturing which temporarily halts the manufacturing process.</cco:definition>
        <rdfs:comment xml:lang="en">This class represents any interruption that occurs during the manufacturing process, causing a temporary halt in production.</rdfs:comment>
        <rdfs:label xml:lang="en">Build Interruption</rdfs:label>
    </owl:Class>
</rdf:RDF>



<!-- Generated by the OWL API (version 4.5.9.2019-02-01T07:24:44Z) https://github.com/owlcs/owlapi -->

